p256: wip: clean up Hacl.Impl.P256.PointMul

code/ecdsap256/Hacl.Impl.P256.PointMul.fst
@@ -1,22 +1,18 @@
 module Hacl.Impl.P256.PointMul
 
+open FStar.Mul
 open FStar.HyperStack.All
 open FStar.HyperStack
 module ST = FStar.HyperStack.ST
-
-open FStar.Mul
-open FStar.Math.Lemmas
 
 open Lib.IntTypes
 open Lib.Buffer
 
 open Hacl.Impl.P256.Bignum
 open Hacl.Impl.P256.Field
-open Hacl.Spec.P256.Math
+open Hacl.Impl.P256.Point
 open Hacl.Impl.P256.PointAdd
 open Hacl.Impl.P256.PointDouble
-open Hacl.Impl.P256.Finv
-open Hacl.Impl.P256.Point
 
 module BSeq = Lib.ByteSequence
 module LSeq = Lib.Sequence
@@ -26,17 +22,12 @@ module SM = Hacl.Spec.P256.MontgomeryMultiplication
 
 #set-options "--z3rlimit 100 --fuel 0 --ifuel 0"
 
-(*This code is taken from Curve25519, written by Polubelova M *)
-val lemma_cswap2_step:
-    bit:uint64{v bit <= 1}
-  -> p1:uint64
-  -> p2:uint64
-  -> Lemma (
-      let mask = u64 0 -. bit in
-      let dummy = mask &. (p1 ^. p2) in
-      let p1' = p1 ^. dummy in
-      let p2' = p2 ^. dummy in
-      if v bit = 1 then p1' == p2 /\ p2' == p1 else p1' == p1 /\ p2' == p2)
+val lemma_cswap2_step: bit:uint64{v bit <= 1} -> p1:uint64 -> p2:uint64 -> Lemma
+  (let mask = u64 0 -. bit in
+   let dummy = mask &. (p1 ^. p2) in
+   let p1' = p1 ^. dummy in
+   let p2' = p2 ^. dummy in
+   if v bit = 1 then p1' == p2 /\ p2' == p1 else p1' == p1 /\ p2' == p2)
 
 let lemma_cswap2_step bit p1 p2 =
   let mask = u64 0 -. bit in
@@ -52,96 +43,25 @@ let lemma_cswap2_step bit p1 p2 =
   let p2' = p2 ^. dummy in
   logxor_lemma p2 p1
 
-(* </> *)
-
-val lemma_scalar_ith: sc:BSeq.lbytes 32 -> k:nat{k < 32} ->
-  Lemma (v (LSeq.index sc k) == BSeq.nat_from_intseq_le sc / pow2 (8 * k) % pow2 8)
-
-let lemma_scalar_ith sc k =
-  BSeq.index_nat_to_intseq_le #U8 #SEC 32 (BSeq.nat_from_intseq_le sc) k;
-  BSeq.nat_from_intseq_le_inj sc (BSeq.nat_to_intseq_le 32 (BSeq.nat_from_intseq_le sc))
-
-
-val lemma_euclidian_for_ithbit: k: nat -> i: nat
-  -> Lemma (k / (pow2 (8 * (i / 8)) * pow2 (i % 8)) == k / pow2 i)
-
-let lemma_euclidian_for_ithbit k i =
-  Math.Lib.lemma_div_def i 8;
-  Math.Lemmas.pow2_plus (8 * (i / 8)) (i % 8)
-
-
-val ith_bit: k:BSeq.lbytes 32 -> i:nat{i < 256}
-  -> t:uint64 {(v t == 0 \/ v t == 1) /\ v t == BSeq.nat_from_intseq_le k / pow2 i % 2}
-
-let ith_bit k i =
-  let open Lib.Sequence in
-  let q = i / 8 in
-  let r = i % 8 in
-  let tmp1 = k.[q] >>. (size r) in
-  let tmp2 = tmp1 &. u8 1 in
-  let res = to_u64 tmp2 in
-  logand_le tmp1 (u8 1);
-  logand_mask tmp1 (u8 1) 1;
-  lemma_scalar_ith k q;
-  let k = BSeq.nat_from_intseq_le k in
-  Math.Lemmas.pow2_modulo_division_lemma_1 (k / pow2 (8 * (i / 8))) (i % 8) 8;
-  Math.Lemmas.division_multiplication_lemma k (pow2 (8 * (i / 8))) (pow2 (i % 8));
-  lemma_euclidian_for_ithbit k i;
-  Math.Lemmas.pow2_modulo_modulo_lemma_1 (k / pow2 i) 1 (8 - (i % 8));
-  res
-
 
 // TODO: rename
 let point_prime = p:point_seq{point_inv_seq p}
 
-val swap: p: point_prime -> q: point_prime -> Tot (r: tuple2 point_prime point_prime {let pNew, qNew = r in
-  pNew == q /\ qNew == p})
-
-let swap p q = (q, p)
+let conditional_swap (i:uint64) (p:point_prime) (q:point_prime) =
+  if uint_v i = 0 then (p, q) else (q, p)
 
 
-val conditional_swap: i: uint64 -> p: point_prime -> q: point_prime -> Tot (r: tuple2 point_prime point_prime
-  {
-    let pNew, qNew = r in
-    if uint_v i = 0 then pNew == p /\ qNew == q
-    else
-      let p1, q1 = swap p q in
-      p1 == pNew /\ q1 == qNew
- }
-)
-
-let conditional_swap i p q =
-  if uint_v i = 0 then
-    (p, q)
-  else
-    (q, p)
-
+val cswap: bit:uint64{v bit <= 1} -> p:point -> q:point -> Stack unit
+  (requires fun h ->
+    live h p /\ live h q /\ eq_or_disjoint p q /\
+    point_inv h p /\ point_inv h q)
+  (ensures  fun h0 _ h1 -> modifies (loc p |+| loc q) h0 h1 /\
+   (let pr, qr = conditional_swap bit (as_seq h0 p) (as_seq h0 q) in
+    as_seq h1 p == pr /\ as_seq h1 q == qr) /\
+    (v bit == 1 ==> as_seq h1 p == as_seq h0 q /\ as_seq h1 q == as_seq h0 p) /\
+    (v bit == 0 ==> as_seq h1 p == as_seq h0 p /\ as_seq h1 q == as_seq h0 q))
 
 [@ CInline]
-val cswap: bit:uint64{v bit <= 1} -> p:point -> q:point
-  -> Stack unit
-    (requires fun h ->
-      live h p /\ live h q /\ (disjoint p q \/ p == q) /\
-
-      as_nat h (gsub p (size 0) (size 4)) < S.prime /\
-      as_nat h (gsub p (size 4) (size 4)) < S.prime /\
-      as_nat h (gsub p (size 8) (size 4)) < S.prime /\
-
-      as_nat h (gsub q (size 0) (size 4)) < S.prime /\
-      as_nat h (gsub q (size 4) (size 4)) < S.prime /\
-      as_nat h (gsub q (size 8) (size 4)) < S.prime
-)
-    (ensures  fun h0 _ h1 ->
-      modifies (loc p |+| loc q) h0 h1 /\
-      (let pBefore = as_seq h0 p in let qBefore = as_seq h0 q in
-  let pAfter = as_seq h1 p in let qAfter = as_seq h1 q in
-  let condP0, condP1 = conditional_swap bit pBefore qBefore  in
-  condP0 == pAfter /\ condP1 == qAfter) /\
-
-      (v bit == 1 ==> as_seq h1 p == as_seq h0 q /\ as_seq h1 q == as_seq h0 p) /\
-      (v bit == 0 ==> as_seq h1 p == as_seq h0 p /\ as_seq h1 q == as_seq h0 q))
-
-
 let cswap bit p1 p2 =
   let open Lib.Sequence in
   let h0 = ST.get () in
@@ -172,129 +92,58 @@ let cswap bit p1 p2 =
 (* this piece of code is taken from Hacl.Curve25519 *)
 (* changed Endian for Scalar Bit access *)
 inline_for_extraction noextract
-val scalar_bit:
-    #buf_type: buftype ->
-    s:lbuffer_t buf_type uint8 (size 32)
-  -> n:size_t{v n < 256}
-  -> Stack uint64
-    (requires fun h0 -> live h0 s)
-    (ensures  fun h0 r h1 -> h0 == h1 /\ r == ith_bit (as_seq h0 s) (v n) /\ v r <= 1)
+val scalar_bit: s:lbuffer uint8 32ul -> n:size_t{v n < 256} -> Stack uint64
+  (requires fun h0 -> live h0 s)
+  (ensures  fun h0 r h1 -> h0 == h1 /\ r == S.ith_bit (as_seq h0 s) (v n) /\ v r <= 1)
 
-let scalar_bit #buf_type s n =
+let scalar_bit s n =
   let h0 = ST.get () in
-  mod_mask_lemma ((Lib.Sequence.index (as_seq h0 s) (31 - v n / 8)) >>. (n %. 8ul)) 1ul;
+  mod_mask_lemma ((LSeq.index (as_seq h0 s) (31 - v n / 8)) >>. (n %. 8ul)) 1ul;
   assert_norm (1 = pow2 1 - 1);
   assert (v (mod_mask #U8 #SEC 1ul) == v (u8 1));
   to_u64 ((s.(31ul -. n /. 8ul) >>. (n %. 8ul)) &. u8 1)
 
 
 inline_for_extraction noextract
-val montgomery_ladder_step1: p: point -> q: point ->tempBuffer: lbuffer uint64 (size 88) -> Stack unit
-  (requires fun h -> live h p /\ live h q /\ live h tempBuffer /\
-    LowStar.Monotonic.Buffer.all_disjoint [loc p; loc q; loc tempBuffer] /\
+val montgomery_ladder_step1: p:point -> q:point -> tmp:lbuffer uint64 (size 88) -> Stack unit
+  (requires fun h ->
+    live h p /\ live h q /\ live h tmp /\
+    disjoint p q /\ disjoint p tmp /\ disjoint q tmp /\
+    point_inv h p /\ point_inv h q)
+  (ensures fun h0 _ h1 -> modifies (loc p |+| loc q |+| loc tmp) h0 h1 /\
+    point_inv h1 p /\ point_inv h1 q /\
+    (SM.from_mont_point (as_point_nat h1 p), SM.from_mont_point (as_point_nat h1 q)) ==
+     S._ml_step1
+      (SM.from_mont_point (as_point_nat h0 p)) (SM.from_mont_point (as_point_nat h0 q)))
 
-    as_nat h (gsub p (size 0) (size 4)) < S.prime /\
-    as_nat h (gsub p (size 4) (size 4)) < S.prime /\
-    as_nat h (gsub p (size 8) (size 4)) < S.prime /\
-
-    as_nat h (gsub q (size 0) (size 4)) < S.prime /\
-    as_nat h (gsub q (size 4) (size 4)) < S.prime /\
-    as_nat h (gsub q (size 8) (size 4)) < S.prime
-
-  )
-  (ensures fun h0 _ h1 -> modifies (loc p |+| loc q |+|  loc tempBuffer) h0 h1 /\
-    (
-      let pX = as_nat h0 (gsub p (size 0) (size 4)) in
-      let pY = as_nat h0 (gsub p (size 4) (size 4)) in
-      let pZ = as_nat h0 (gsub p (size 8) (size 4)) in
-
-      let qX = as_nat h0 (gsub q (size 0) (size 4)) in
-      let qY = as_nat h0 (gsub q (size 4) (size 4)) in
-      let qZ = as_nat h0 (gsub q (size 8) (size 4)) in
-
-      let r0X = as_nat h1 (gsub p (size 0) (size 4)) in
-      let r0Y = as_nat h1 (gsub p (size 4) (size 4)) in
-      let r0Z = as_nat h1 (gsub p (size 8) (size 4)) in
-
-      let r1X = as_nat h1 (gsub q (size 0) (size 4)) in
-      let r1Y = as_nat h1 (gsub q (size 4) (size 4)) in
-      let r1Z = as_nat h1 (gsub q (size 8) (size 4)) in
-
-
-      let (rN0X, rN0Y, rN0Z), (rN1X, rN1Y, rN1Z) = S._ml_step1 (SM.from_mont pX, SM.from_mont pY, SM.from_mont pZ) (SM.from_mont qX, SM.from_mont qY, SM.from_mont qZ) in
-
-      SM.from_mont r0X == rN0X /\ SM.from_mont r0Y == rN0Y /\ SM.from_mont r0Z == rN0Z /\
-      SM.from_mont r1X == rN1X /\ SM.from_mont r1Y == rN1Y /\ SM.from_mont r1Z == rN1Z /\
-
-      r0X < S.prime /\ r0Y < S.prime /\ r0Z < S.prime /\
-      r1X < S.prime /\ r1Y < S.prime /\ r1Z < S.prime
-  )
-)
-
-
-let montgomery_ladder_step1 r0 r1 tempBuffer =
-  point_add r0 r1 r1 tempBuffer;
-  point_double r0 r0 tempBuffer
-
-
-val lemma_step: i: size_t {uint_v i < 256} -> Lemma  (uint_v ((size 255) -. i) == 255 - (uint_v i))
-let lemma_step i = ()
+let montgomery_ladder_step1 r0 r1 tmp =
+  point_add r0 r1 r1 tmp;
+  point_double r0 r0 tmp
 
 
 inline_for_extraction noextract
-val montgomery_ladder_step: #buf_type: buftype->
-  p: point -> q: point ->tempBuffer: lbuffer uint64 (size 88) ->
-  scalar: lbuffer_t buf_type uint8 (size 32) ->
-  i:size_t{v i < 256} ->
+val montgomery_ladder_step:
+    p:point -> q:point -> tmp:lbuffer uint64 88ul
+  -> scalar:lbuffer uint8 32ul
+  -> i:size_t{v i < 256} ->
   Stack unit
-  (requires fun h -> live h p /\ live h q /\ live h tempBuffer /\ live h scalar /\
-    LowStar.Monotonic.Buffer.all_disjoint [loc p; loc q; loc tempBuffer; loc scalar] /\
+  (requires fun h ->
+    live h p /\ live h q /\ live h tmp /\ live h scalar /\
+    LowStar.Monotonic.Buffer.all_disjoint [loc p; loc q; loc tmp; loc scalar] /\
+    point_inv h p /\ point_inv h q)
+  (ensures fun h0 _ h1 -> modifies (loc p |+| loc q |+| loc tmp) h0 h1 /\
+    point_inv h1 p /\ point_inv h1 q /\
+    (SM.from_mont_point (as_point_nat h1 p), SM.from_mont_point (as_point_nat h1 q)) ==
+     S._ml_step (as_seq h0 scalar) (v i)
+      (SM.from_mont_point (as_point_nat h0 p), SM.from_mont_point (as_point_nat h0 q)))
 
-    as_nat h (gsub p (size 0) (size 4)) < S.prime /\
-    as_nat h (gsub p (size 4) (size 4)) < S.prime /\
-    as_nat h (gsub p (size 8) (size 4)) < S.prime /\
-
-    as_nat h (gsub q (size 0) (size 4)) < S.prime /\
-    as_nat h (gsub q (size 4) (size 4)) < S.prime /\
-    as_nat h (gsub q (size 8) (size 4)) < S.prime
-  )
-  (ensures fun h0 _ h1 -> modifies (loc p |+| loc q |+| loc tempBuffer) h0 h1 /\
-    (
-
-      let pX = as_nat h0 (gsub p (size 0) (size 4)) in
-      let pY = as_nat h0 (gsub p (size 4) (size 4)) in
-      let pZ = as_nat h0 (gsub p (size 8) (size 4)) in
-
-      let qX = as_nat h0 (gsub q (size 0) (size 4)) in
-      let qY = as_nat h0 (gsub q (size 4) (size 4)) in
-      let qZ = as_nat h0 (gsub q (size 8) (size 4)) in
-
-      let r0X = as_nat h1 (gsub p (size 0) (size 4)) in
-      let r0Y = as_nat h1 (gsub p (size 4) (size 4)) in
-      let r0Z = as_nat h1 (gsub p (size 8) (size 4)) in
-
-      let r1X = as_nat h1 (gsub q (size 0) (size 4)) in
-      let r1Y = as_nat h1 (gsub q (size 4) (size 4)) in
-      let r1Z = as_nat h1 (gsub q (size 8) (size 4)) in
-
-      let (rN0X, rN0Y, rN0Z), (rN1X, rN1Y, rN1Z) = S._ml_step (as_seq h0 scalar) (uint_v i) ((SM.from_mont pX, SM.from_mont pY, SM.from_mont pZ), (SM.from_mont qX, SM.from_mont qY, SM.from_mont qZ)) in
-
-      SM.from_mont r0X == rN0X /\ SM.from_mont r0Y == rN0Y /\ SM.from_mont r0Z == rN0Z /\
-      SM.from_mont r1X == rN1X /\ SM.from_mont r1Y == rN1Y /\ SM.from_mont r1Z == rN1Z /\
-
-      r0X < S.prime /\ r0Y < S.prime /\ r0Z < S.prime /\
-      r1X < S.prime /\ r1Y < S.prime /\ r1Z < S.prime
-    )
-  )
-
-
-let montgomery_ladder_step #buf_type r0 r1 tempBuffer scalar i =
-  let bit0 = (size 255) -. i in
+let montgomery_ladder_step r0 r1 tmp scalar i =
+  let bit0 = 255ul -. i in
+  assert (v bit0 = 255 - v i);
   let bit = scalar_bit scalar bit0 in
   cswap bit r0 r1;
-  montgomery_ladder_step1 r0 r1 tempBuffer;
-  cswap bit r0 r1;
-    lemma_step i
+  montgomery_ladder_step1 r0 r1 tmp;
+  cswap bit r0 r1
 
 
 val montgomery_ladder: p:point -> q:point
